src/implementations/intfrac_rationals.v
@@ -4,4 +4,4 @@ Require Import
   abstract_algebra field_of_fractions theory.rationals.
 
 Instance intfrac_rationals `{Integers Z} `{∀ x y: Z, Decision (x = y)} : Rationals (Frac Z).
-Proof. apply (alt_Build_Rationals _ _ _ _ _). Qed.
+Proof alt_Build_Rationals _.
