src/theory/bit_shift.v
@@ -1,68 +1,74 @@
 Require
-  theory.naturals theory.integers orders.orders.
+  orders.integers theory.fields.
 Require Import 
   Program Morphisms Setoid Ring
   abstract_algebra interfaces.naturals interfaces.integers interfaces.additional_operations
-  theory.nat_pow.
+  theory.nat_pow theory.int_pow.
 
-(* * Properties of Shift Left *)
-Section shift_left_properties.
-  Context `{SemiRing A} `{Naturals B} `{!NatPow A B} `{sl : !ShiftLeft A B}.
-
-  Lemma shiftl_correct x y : x ≪ y = x * 2  ^ y.
-  Proof.
-    unfold shiftl. unfold shiftl_sig. 
-    destruct sl. simpl. auto.
-  Qed.
-
-  Global Instance shiftl_proper: Proper ((=) ==> (=) ==> (=)) (≪).
-  Proof. 
-    intros x1 y1 E1 x2 y2 E2. 
-    rewrite (shiftl_correct x1 x2). rewrite (shiftl_correct y1 y2).
-    rewrite E1, E2. reflexivity. 
-  Qed.
+(* * Properties of [shiftl] on the naturals *)
+Section shift_left_naturals.
+  Context `{SemiRing A} `{Naturals B}.
 
   Add Ring A2: (rings.stdlib_semiring_theory A).
   Add Ring B2: (rings.stdlib_semiring_theory B).
 
-  Global Instance: LeftAbsorb (≪) 0.
-  Proof. intro. rewrite shiftl_correct. ring. Qed.
+  Lemma shiftl_spec_from_nat_pow `{!NatPowSpec A B np} (sl : ShiftL A B) :
+    (∀ x n, x ≪ n = x * 2 ^ n) → ShiftLSpec A B sl.
+  Proof.
+    intros spec.
+    split.
+      intros ? ? E1 ? ? E2.
+      do 2 rewrite spec. now rewrite E1, E2.
+     intro x. rewrite spec, nat_pow_0. ring.
+    intros x n. do 2 rewrite spec. rewrite nat_pow_S. ring.
+  Qed.
 
-  Global Instance: RightIdentity (≪) 0.
-  Proof. intro. rewrite shiftl_correct. rewrite nat_pow_0. ring. Qed.
+  Context `{!ShiftLSpec A B sl}.
+
+  Global Instance: Proper ((=) ==> (=) ==> (=)) (≪) | 1.
+  Proof. apply shiftl_proper. Qed.
+
+  Lemma shiftl_nat_pow `{!NatPowSpec A B np} x n : x ≪ n = x * 2 ^ n.
+  Proof.
+    revert n. apply naturals.induction.
+      intros ? ? E1. rewrite E1. reflexivity.
+     rewrite nat_pow_0. do 2 rewrite right_identity. reflexivity.
+    intros ? E. rewrite nat_pow_S, shiftl_S, E. ring.
+  Qed.
+
+  Global Instance: LeftAbsorb (≪) 0.
+  Proof. intro. rewrite shiftl_nat_pow. ring. Qed.
 
   Lemma shiftl_order x y z: x ≪ y ≪ z  = x ≪ z ≪ y.
-  Proof. do 4 rewrite shiftl_correct. ring. Qed.
+  Proof. do 4 rewrite shiftl_nat_pow. ring. Qed.
 
   Lemma shiftl_order_4a x y1 y2 y3: x ≪ y1 ≪ y2 ≪ y3  = x ≪ y3 ≪ y2 ≪ y1.
-  Proof. do 6 rewrite shiftl_correct. ring. Qed.
+  Proof. do 6 rewrite shiftl_nat_pow. ring. Qed.
 
   Lemma shiftl_order_4b x y1 y2 y3: x ≪ y1 ≪ y2 ≪ y3  = x ≪ y2 ≪ y3 ≪ y1.
-  Proof. do 6 rewrite shiftl_correct. ring. Qed.
+  Proof. do 6 rewrite shiftl_nat_pow. ring. Qed.
 
   Lemma mult_shiftl x y z: x * (y ≪ z) = (x * y) ≪ z.
-  Proof. do 2 rewrite shiftl_correct. ring. Qed.
+  Proof. do 2 rewrite shiftl_nat_pow. ring. Qed.
 
   Lemma mult_shiftl_1 x y: x ≪ y = x * (1 ≪ y).
-  Proof. do 2 rewrite shiftl_correct. ring. Qed.
+  Proof. do 2 rewrite shiftl_nat_pow. ring. Qed.
 
-  Lemma shiftl_sum_base x y z: (x + y) ≪ z  = x ≪ z + y ≪ z.
-  Proof. do 3 rewrite shiftl_correct. ring. Qed.
+  Lemma shiftl_plus_base x y z: (x + y) ≪ z  = x ≪ z + y ≪ z.
+  Proof. do 3 rewrite shiftl_nat_pow. ring. Qed.
 
-  Lemma shiftl_sum_exp x y z: x ≪ (y + z) = x ≪ y ≪ z.
-  Proof. do 3 rewrite shiftl_correct. rewrite nat_pow_exp_plus. ring. Qed.
+  Lemma shiftl_plus_exp x y z: x ≪ (y + z) = x ≪ y ≪ z.
+  Proof. do 3 rewrite shiftl_nat_pow. rewrite nat_pow_exp_plus. ring. Qed.
 
   Lemma mult_r_shiftl_shiftl x y z1 z2 : (x * (y ≪ z1)) ≪ z2 = (x * y) ≪ (z1 + z2).
-  Proof. do 3 rewrite shiftl_correct. rewrite nat_pow_exp_plus. ring. Qed.
+  Proof. do 3 rewrite shiftl_nat_pow. rewrite nat_pow_exp_plus. ring. Qed.
 
   Lemma mult_l_shiftl_shiftl x y z1 z2 : ((x ≪ z1) * y) ≪ z2 = (x * y) ≪ (z1 + z2).
-  Proof. do 3 rewrite shiftl_correct. rewrite nat_pow_exp_plus. ring. Qed.
+  Proof. do 3 rewrite shiftl_nat_pow. rewrite nat_pow_exp_plus. ring. Qed.
 
-  Context `{GroupInv A} .
-
-  Lemma opp_shiftl `{!Ring A} x y : (-x) ≪ y = -(x ≪ y).
+  Lemma opp_shiftl `{GroupInv A} `{!Ring A} x y : (-x) ≪ y = -(x ≪ y).
   Proof.
-    do 2 rewrite shiftl_correct.
+    do 2 rewrite shiftl_nat_pow.
     rewrite rings.opp_mult. symmetry. rewrite rings.opp_mult at 1.
     ring.
   Qed.
@@ -71,7 +77,7 @@ Section shift_left_properties.
 
   Lemma shiftl_nonzero x y: x ≠ 0 → x ≪ y ≠ 0.
   Proof with auto.
-    intros E1 E2. rewrite shiftl_correct in E2. 
+    intros E1 E2. rewrite shiftl_nat_pow in E2. 
     apply (no_zero_divisors x). split... 
     exists (2 ^ y); split...
     apply nat_pow_nonzero.
@@ -82,160 +88,44 @@ Section shift_left_properties.
   Lemma shiftl_inj n : Injective (flip shiftl n).
   Proof with auto.
     repeat (split; try apply _).
-    intros x y E. unfold flip in E. do 2 rewrite shiftl_correct in E.
+    intros x y E. unfold flip in E. do 2 rewrite shiftl_nat_pow in E.
     apply (rings.right_cancellation_ne_0 (.*.) (2 ^ n))...
     apply nat_pow_nonzero. apply (ne_zero 2).
   Qed.
-End shift_left_properties.
+End shift_left_naturals.
 
-(* * Default Shift Left implementation using Nat Pow*)
-Global Program Instance default_shiftl `{SemiRing A} `{Naturals B} `{!NatPow A B} : ShiftLeft A B | 10 
-  := λ x y, x * 2 ^ y.
-Next Obligation. reflexivity. Qed.
+Section default_shiftl.
+  Context `{SemiRing A} `{Naturals B} `{!NatPowSpec A B pw}.
 
-(*
-(* * Properties of Shift Right *)
-Section shift_right_properties.
-  Context `{SemiRing A} `{Naturals B}.
-  Context `{!NatPow A B} 
-    `{sr : !ShiftRight A B}
-    `{sl : !ShiftLeft A B}
-    `{!NoZeroDivisors A} 
-    `{!NeZero (1:A)} 
-    `{!NeZero (2:A)} 
-    `{!∀ z, NeZero z → LeftCancellation (.*.) z}.
+  Global Instance default_shiftl: ShiftL A B := λ x n, x * 2 ^ n.
 
-  Hint Resolve orders.strictly_precedes_weaken.
+  Global Instance: ShiftLSpec A B default_shiftl.
+  Proof. now apply shiftl_spec_from_nat_pow. Qed.
+End default_shiftl.
 
-  Lemma shiftr_correct (x : A) y : x ≤ (x ≫ y) * 2 ^ y < 2 * x.
-  Proof.
-    unfold shiftr. unfold shiftr_sig. 
-    destruct sr. simpl. assumption.
+Section shift_left_integers.
+  Context `{Field A} `{Integers B} `{!ShiftLSpec A B sl} `{∀ x y : A, Decision (x = y)} `{!IntPowSpec A B ipw} `{!NeZero (2:A)}.
+
+  Add Ring A: (rings.stdlib_semiring_theory A).
+  Add Ring B: (rings.stdlib_ring_theory B).
+
+  Global Instance: Proper ((=) ==> (=) ==> (=)) (≪) | 1.
+  Proof. apply shiftl_proper. Qed.
+
+  Lemma shiftl_int_pow x n : x ≪ n = x * 2 ^ n.
+  Proof. 
+    revert n. apply integers.induction.
+       solve_proper.
+      rewrite shiftl_0, int_pow_0. ring.
+     intros n E1 E2. rewrite shiftl_S, E2, int_pow_S. ring.
+     apply (ne_zero (2:A)). 
+    intros n E1 E2.
+    apply (left_cancellation (.*.) 2).
+    rewrite <-shiftl_S.
+    setoid_replace (1 + (n - 1)) with n by ring.
+    rewrite E2.
+    setoid_replace n with (1 + (n - 1)) at 1 by ring.
+    rewrite int_pow_S. ring.
+    apply (ne_zero (2:A)).
   Qed.
-  
-  Lemma shiftr_shiftl_correct (x : A) y : x ≤ (x ≫ y) ≪ y < 2 * x.
-  Proof.
-    rewrite shiftl_correct. apply shiftr_correct. 
-  Qed.
-End shift_right_properties.
-
-  Lemma shiftl_shiftr_correct x y : x = (x ≪ y) ≫ y.
-  Proof with auto.
-    unfold shiftr. unfold shiftr_sig. 
-    destruct sr as [z [E1 E2]]. simpl.
-    apply (right_cancellation (≪) y). unfold flip.
-    rewrite <-shiftl_correct in E1, E2. 
-    apply (antisymmetry (≤))...
-  Qed.
-
-  Global Instance shiftr_proper: Proper ((=) ==> (=) ==> (=)) shiftr.
-  Proof with auto. 
-    intros x1 x2 E y1 y2 F. 
-    unfold shiftr. unfold shiftr_sig. 
-    destruct (sr x1 y1) as [z1 [Ez1 Fz1]], (sr x2 y2) as [z2 [Ez2 Fz2]]. simpl.
-    rewrite F in Ez1, Fz1. 
-    apply (rings.mult_injective (2 ^ y2)).
-      apply nat_pow_nonzero, integers.two_nonzero.
-    rewrite commutativity. symmetry. rewrite commutativity.
-    transitivity x2. apply (antisymmetry (≤))...
-    transitivity x1. symmetry... apply (antisymmetry (≤))...
-  Qed.
-
-  Add Ring A3: (rings.stdlib_semiring_theory A).
-  Add Ring B3: (rings.stdlib_semiring_theory B).
-
-  Global Instance: LeftAbsorb shiftr 0.
-  Proof with auto; try reflexivity. 
-    intros x. assert (0 = 0 ≪ x) as E. rewrite left_absorb...
-    rewrite E at 1. symmetry. apply shiftl_shiftr_correct.
-  Qed.  
-
-  Global Instance: RightIdentity shiftr 0.
-  Proof with auto; try reflexivity. 
-    intros x. assert (x = x ≪ 0) as E. rewrite right_identity...
-    rewrite E at 1. symmetry. apply shiftl_shiftr_correct.
-  Qed.
-
-  Lemma shiftr_sum_exp x y z: x ≫ (y + z) = x ≫ y ≫ z.
-  Proof with auto; try reflexivity. 
-    unfold shiftr. unfold shiftr_sig. 
-    destruct (sr x y) as [z1 [Ez1 Fz1]]. simpl. 
-    destruct (sr z1 z) as [z2 [Ez2 Fz2]]. simpl. 
-    set (p:=(_ : RingPlus B)). (* why can't do this properly? *)
-    destruct (sr x (@ring_plus B p y z)) as [z3 [Ez3 Fz3]]. simpl.
-    apply (rings.mult_injective (2 ^ (y + z))).
-      apply nat_pow_nonzero, integers.two_nonzero.
-    rewrite commutativity. symmetry. rewrite commutativity. symmetry.
-    transitivity x. apply (antisymmetry (≤))...
-
-  Lemma shiftr_order x y z: x ≫ y ≫ z  = x ≫ z ≫ y.
-  Proof with auto; try reflexivity.
-    unfold shiftr. unfold shiftr_sig. 
-    destruct (sr x y) as [z1 [Ez1 Fz1]], (sr x z) as [z2 [Ez2 Fz2]]. simpl.
-    destruct (sr z1 z) as [z3 [Ez3 Fz3]], (sr z2 y) as [z4 [Ez4 Fz4]]. simpl.
-
-  Lemma shiftr_order_4a x y1 y2 y3: x ≪ y1 ≪ y2 ≪ y3  = x ≪ y3 ≪ y2 ≪ y1.
-  Proof. do 6 rewrite shiftl_correct. ring. Qed.
-
-  Lemma shiftr_order_4b x y1 y2 y3: x ≪ y1 ≪ y2 ≪ y3  = x ≪ y2 ≪ y3 ≪ y1.
-  Proof. do 6 rewrite shiftl_correct. ring. Qed.
-
-  Lemma mult_shiftr x y z: x * (y ≪ z) = (x * y) ≪ z.
-  Proof. do 2 rewrite shiftl_correct. ring. Qed.
-
-  Lemma mult_shiftr_1 x y: x ≪ y = x * (1 ≪ y).
-  Proof. do 2 rewrite shiftl_correct. ring. Qed.
-
-  Lemma shiftr_sum_base x y z: (x + y) ≪ z  = x ≪ z + y ≪ z.
-  Proof. do 3 rewrite shiftl_correct. ring. Qed.
-
-  Lemma shiftr_sum_exp x y z: x ≪ (y + z) = x ≪ y ≪ z.
-  Proof. do 3 rewrite shiftl_correct. rewrite nat_pow_exp_sum. ring. Qed.
-
-  Context `{GroupInv A} .
-
-  Lemma opp_shiftr `{!Ring A} x y : (-x) ≪ y = -(x ≪ y).
-  Proof.
-    do 2 rewrite shiftl_correct.
-    rewrite rings.ring_opp_mult. symmetry. rewrite rings.ring_opp_mult at 1.
-    ring.
-  Qed.
-
-  Context `{IntegersToRing A} `{!Integers A}.
-
-  Lemma shiftr_nonzero x y: x ≠ 0 → x ≪ y ≠ 0.
-  Proof with auto.
-    intros E1 E2. rewrite shiftl_correct in E2. 
-    apply (no_zero_divisors x). split... 
-    exists (2 ^ y); split...
-    apply nat_pow_nonzero.
-    apply integers.two_nonzero.
-  Qed.
-
-  (* x ≪ b = y ≪ b → x = y *)
-  Lemma shiftr_inj n : Injective (flip shiftl n).
-  Proof.
-    repeat (split; try apply _).
-    intros x y E. unfold flip in E. do 2 rewrite shiftl_correct in E.
-    apply rings.mult_injective with (2 ^ n).
-    apply nat_pow_nonzero, integers.two_nonzero.
-    rewrite commutativity, E. ring.
-  Qed. 
-End shift_right_properties.  
-
-(* * Default Shift Left implementation using Nat Pow*)
-Section default_shiftr.
-  Context `{SemiRing A} 
-    `{Naturals B} 
-    `{!NatPow A B} 
-    `{!DivEuclid A} 
-    `{!NoZeroDivisors A} 
-    `{!NeZero (1:A)}
-    `{!NeZero (2:A)}
-
-  Global Program Instance default_shiftr : ShiftRight A B | 10 
-    := λ x y, div_euclid x (exist _ (2 ^ y) _).
-  Next Obligation. eapply nat_pow_nonzero. apply (ne_zero 2). Qed.
-  Next Obligation. admit. Qed.
-End default_shiftr.
-*)
+End shift_left_integers.
