src/theory/int_pow.v
@@ -7,157 +7,109 @@ Require Import
 
 (* * Properties of Int Pow *)
 Section int_pow_properties.
-Context `{Field A} 
-  `{∀ z, NeZero z → LeftCancellation (.*.) z}
-  `{∀ x y, Decision (x = y)} `{!DecMultInv A}
-  `{Integers B} `{oB : Order B} `{!RingOrder oB} `{!TotalOrder oB}.
+Context `{Field A} `{∀ x y, Decision (x = y)} `{!DecMultInv A}
+  `{Integers B} `{oB : Order B} `{!RingOrder oB} `{!TotalOrder oB} `{!IntPowSpec A B ipw}.
 
-Add Ring A : (rings.stdlib_semiring_theory A).
+Add Ring A : (rings.stdlib_ring_theory A).
 Add Ring B : (rings.stdlib_ring_theory B).
 
-Section int_pow_spec_from_properties.
-  Context (f : A → B → A) {f_proper : Proper ((=) ==> (=) ==> (=)) f}
-    ( f_0 : ∀x, f x 0 = 1 ) ( f_S : ∀ x n, 0 ≤ n → f x (1+n) = x * (f x n) ).
-
-  Lemma int_pow_spec_from_properties_nonneg x n : 0 ≤ n → nat_pow_spec x n (f x n).
-  Proof with auto; try reflexivity.
-    intros E. pattern n. apply integers.induction_nonneg...
-      intros a b F. 
-      eapply nat_pow_spec_proper...
-      rewrite F...
-     eapply nat_pow_spec_proper... apply nat_pow_spec_0...
-    intros. eapply nat_pow_spec_proper...
-    eapply nat_pow_spec_S...
-  Qed.
-
-  Context ( f_inv : ∀ x n,  f x (-n) = /(f x n) ).
-  Lemma int_pow_spec_from_properties x n : 
-    (0 ≤ n → nat_pow_spec x n (f x n)) ∧ (n ≤ 0 → nat_pow_spec x (-n) (/ (f x n))).
-  Proof with trivial.
-    split.
-     apply int_pow_spec_from_properties_nonneg.
-    intros. eapply (nat_pow_spec_proper _ _ (reflexivity _) _ _ (reflexivity _)).
-     symmetry...
-    apply int_pow_spec_from_properties_nonneg.
-    apply rings.flip_nonpos_inv...
-  Qed.
-End int_pow_spec_from_properties.
-
-Context `{ip : !IntPow A B}.
-Global Instance: Proper ((=) ==> (=) ==> (=)) (^).
-Proof with eauto.
-  intros x y E1 n m E2. 
-  unfold pow, int_pow, int_pow_sig. 
-  destruct ip as [z1 [Ez1 Fz1]], ip as [z2 [Ez2 Fz2]]. simpl.
-  destruct (total_order 0 n).
-   eapply nat_pow_spec_unique...
-   eapply nat_pow_spec_proper... reflexivity.
-   apply Ez2. rewrite <-E2...
-  apply (injective (/)).
-  eapply nat_pow_spec_unique...
-  eapply nat_pow_spec_proper... apply inv_proper... 
-  reflexivity.
-  apply Fz2. rewrite <-E2...
-Qed.
-
-Lemma int_pow_0 x : x ^ (0:B) = 1.
-Proof with eauto.
-  unfold pow, int_pow, int_pow_sig. destruct ip as [z [Fz Gz]]. simpl.
-  eapply nat_pow_spec_unique. 
-  apply Fz. reflexivity.
-  apply nat_pow_spec_0.
-Qed.
-
-Lemma int_pow_mult_inv (x : A) (n : B) : x ^(-n) = /(x ^ n).
-Proof with auto.
-  unfold pow, int_pow, int_pow_sig. 
-  destruct (ip x n) as [z2 [Ez2 Fz2]]. destruct ip as [z1 [Ez1 Fz1]]. simpl.
-  destruct (total_order 0 n).
-   apply (injective (/)).
-   eapply nat_pow_spec_unique.
-    apply Fz1, rings.flip_nonneg_inv...
-   eapply (nat_pow_spec_proper _ _ (reflexivity _)).
-     apply rings.inv_involutive.
-    apply fields.dec_mult_inv_involutive.
-   apply Ez2...
-  eapply nat_pow_spec_unique.
-   apply Ez1, rings.flip_nonpos_inv...
-  apply Fz2...
-Qed.
-
-Lemma int_pow_mult_inv_alt (x : A) (n : B) : x ^n = /(x ^ (-n)).
-Proof.
-  rewrite <-int_pow_mult_inv.
-  rewrite rings.inv_involutive.
-  reflexivity.
-Qed.
+Global Instance: Proper ((=) ==> (=) ==> (=)) (^) | 1.
+Proof. apply int_pow_proper. Qed.
 
 Lemma int_pow_S_nonneg (x : A) (n : B) : 0 ≤ n → x ^ (1+n) = x * x ^ n.
-Proof with eauto.
-  intros E.
-  unfold pow, int_pow, int_pow_sig. 
-  destruct ip as [z1 [F1 G1]], ip as [z2 [F2 G2]]. simpl.
-  eapply nat_pow_spec_unique. 
-  apply F1. apply semirings.nonneg_plus_compat...
-   apply semirings.precedes_0_1...
-  apply nat_pow_spec_S...
+Proof.
+  intros E1.
+  destruct (decide (x = 0)) as [Ex|Ex].
+   rewrite Ex. rewrite int_pow_base_0. ring.
+   intros E2. destruct semirings.not_precedes_1_0. 
+   rewrite <-E2. now apply semirings.nonneg_plus_compat_r.
+  now rewrite int_pow_S.
 Qed.
 
-Lemma int_pow_S (x : A) (n : B) : x ≠ 0 →  x ^ (1+n) = x * x ^ n.
-Proof with auto.
-  intros E.
-  destruct (orders.precedes_or_sprecedes 0 n).
-   apply int_pow_S_nonneg...
-   rewrite int_pow_mult_inv_alt, (int_pow_mult_inv_alt _ n).
-  setoid_replace (-n) with (1 - (1 + n)) by ring.
-  rewrite int_pow_S_nonneg.
-  rewrite fields.dec_mult_inv_distr. rewrite associativity. 
-  rewrite fields.dec_mult_inverse... ring.
-  apply rings.flip_nonpos_inv...
-  rewrite commutativity.
-  apply integers.precedes_sprecedes_alt...
+Lemma int_pow_mult_inv (x : A) (n : B) : x ^ (-n) = /(x ^ n).
+Proof with auto; try reflexivity.
+  pattern n. apply integers.induction; clear n.
+     solve_proper.
+    now rewrite rings.opp_0, int_pow_0, fields.dec_mult_inv_1.
+   intros n E1 E2.
+   rewrite int_pow_S_nonneg, fields.dec_mult_inv_distr, <-E2...
+   destruct (decide (x = 0)) as [E3|E3].
+    rewrite E3, int_pow_base_0, fields.dec_mult_inv_0. ring.
+    rewrite commutativity. apply rings.flip_opp_nonzero. apply not_symmetry.
+    apply integers.precedes_sprecedes in E1. now destruct E1.
+   apply (rings.left_cancellation_ne_0 (.*.) x)...
+   rewrite <-int_pow_S...
+   setoid_replace (1 - (1 + n)) with (-n) by ring.
+   rewrite associativity, fields.dec_mult_inverse... ring.
+  intros n E1 E2.
+  setoid_replace (-(n - 1)) with (1 + -n) by ring.
+  rewrite int_pow_S_nonneg, E2...
+   destruct (decide (x = 0)) as [E3|E3].
+    rewrite E3, left_absorb.
+    rewrite int_pow_base_0, fields.dec_mult_inv_0...
+    intros E4. destruct semirings.not_precedes_1_0. 
+    apply rings.flip_nonpos_inv.
+    apply (order_preserving_back (n +)). 
+    rewrite E4. now ring_simplify.
+   apply (rings.left_cancellation_ne_0 (.*.) (/x))...
+    now apply fields.dec_mult_inv_nonzero.
+   rewrite <-fields.dec_mult_inv_distr, <-int_pow_S...
+   setoid_replace (1 + (n - 1)) with n by ring.
+   rewrite associativity, (commutativity (/x)), fields.dec_mult_inverse... ring.
+  now apply rings.flip_nonpos_inv.
 Qed.
 
-Lemma int_pow_nat_pow `{Naturals N} `{!NatPow A N} (x : A) (n : N) :
-  x ^ (naturals_to_semiring N B n) = x ^ n.
+Lemma int_pow_mult_inv_alt (x : A) (n : B) : x ^ n = /(x ^ (-n)).
+Proof.
+  rewrite <-int_pow_mult_inv.
+  now rewrite rings.inv_involutive.
+Qed.
+
+Lemma int_pow_nat_pow `{Naturals N} `{!NatPowSpec A N pw} {f : N → B} `{!SemiRing_Morphism f} (x : A) (n : N) :
+  x ^ (f n) = x ^ n.
 Proof.
   revert n. apply naturals.induction.
-    intros ? ? E. rewrite E. reflexivity.
-   rewrite rings.preserves_0, int_pow_0, nat_pow_0. reflexivity.
+    solve_proper.
+   now rewrite rings.preserves_0, int_pow_0, nat_pow_0.
   intros n E.
   rewrite rings.preserves_plus, rings.preserves_1.
   rewrite int_pow_S_nonneg, nat_pow_S.
-   rewrite E. reflexivity.
-  apply naturals.to_semiring_nonneg.
+   now rewrite E.
+  rewrite <-(rings.preserves_0 (f:=f)).
+  apply (order_preserving _).
+  now apply naturals.naturals_nonneg.
 Qed.
 
 Instance: RightIdentity (^) (1:B).
 Proof. 
   intro. assert ((1:B) = 1 + 0) as E by ring. rewrite E.
-  rewrite int_pow_S_nonneg, int_pow_0. ring.
+  rewrite int_pow_S_nonneg, int_pow_0. 
+   ring.
   reflexivity.
 Qed.
 
-Instance: LeftAbsorb (pow (B:=B)) (1 : A).
+Instance: LeftAbsorb (^) 1.
 Proof with auto. 
   intro n. 
   pattern n. apply integers.induction; clear n.
-     intros ? ? E. rewrite E. tauto.
-    apply int_pow_0.
+     solve_proper.
+    now apply int_pow_0.
    intros n E F.
-   rewrite int_pow_S_nonneg... rewrite F. ring.
+   rewrite int_pow_S_nonneg... 
+   rewrite F. ring.
   intros n E F. 
   setoid_replace n with (1 + (n - 1)) in F by ring.
-  rewrite int_pow_S in F. ring_simplify in F...
-  apply (ne_zero 1).
+  rewrite int_pow_S in F. 
+   now ring_simplify in F.
+  now apply (ne_zero 1).
 Qed.
 
-Lemma int_pow_exp_sum (n m: B) (x : A) : 
+Lemma int_pow_exp_plus (n m : B) (x : A) : 
   x ≠ 0 → x ^ (n + m) = x ^ n * x ^ m.
 Proof with auto.
   intros nonneg.
   pattern n. apply integers.induction; clear n.
-     intros ? ? E. rewrite E. tauto.
+     solve_proper.
     rewrite int_pow_0, left_identity. ring.
    intros ? ? E. 
    rewrite <-associativity.
@@ -172,21 +124,21 @@ Qed.
 Lemma int_pow_of_0 (n : B) : n ≠ 0 → 0 ^ n = 0.
 Proof with auto.
   pattern n. apply integers.induction; clear n.
-     intros ? ? E. rewrite E. tauto.
-    intro E. destruct E. reflexivity.
+     solve_proper.
+    intro E. now destruct E.
    intros. rewrite int_pow_S_nonneg... ring.
   intros n ? ? ?. rewrite int_pow_mult_inv_alt.
   setoid_replace (-(n - 1)) with (1 - n) by ring.
   rewrite int_pow_S_nonneg. 
    rewrite left_absorb. apply fields.dec_mult_inv_0.
-  apply rings.flip_nonpos_inv...
+  now apply rings.flip_nonpos_inv.
 Qed.
 
 Lemma int_pow_nonzero (x : A) (n : B) : x ≠ 0 → x ^ n ≠ 0.
 Proof with eauto.
   intros nonneg.
   pattern n. apply integers.induction; clear n.
-     intros x1 x2 E. rewrite E. reflexivity.
+     solve_proper.
     intros. rewrite int_pow_0. apply (ne_zero 1).
    intros n E1 ? E2. rewrite int_pow_S_nonneg in E2...
    apply (no_zero_divisors x); split...
@@ -197,11 +149,11 @@ Qed.
 
 Context `{oA : Order A} `{!RingOrder oA} `{!TotalOrder oA}.
 
-Lemma int_pow_nonneg (x : A) (n : B) : 0 < x → 0 < x ^ n.
+Lemma int_pow_pos (x : A) (n : B) : 0 < x → 0 < x ^ n.
 Proof with auto.
   intros nonneg.
   pattern n. apply integers.induction; clear n.
-     intros x1 x2 E. rewrite E. reflexivity.
+     solve_proper.
     intros. rewrite int_pow_0. apply semirings.sprecedes_0_1.
    intros n E1 E2. rewrite int_pow_S_nonneg...
    apply semirings.pos_mult_compat...
@@ -212,13 +164,61 @@ Proof with auto.
    rewrite right_absorb. setoid_replace (1 + (n - 1)) with n by ring...
   apply not_symmetry. apply orders.neq_precedes_sprecedes...
 Qed. 
+
+Lemma int_pow_nonneg (x : A) (n : B) : 0 ≤ x → 0 ≤ x ^ n.
+Proof with auto.
+  intros E.
+  apply orders.sprecedes_precedes in E.
+  destruct E as [E|E].
+   rewrite <-E.
+   destruct (decide (n = 0)) as [E2|E2].
+    rewrite E2.
+    rewrite int_pow_0.
+    apply semirings.precedes_0_1.
+   now rewrite int_pow_of_0.
+  now apply int_pow_pos.
+Qed. 
+
+Lemma int_pow_ge1 (x : A) (n : B) : 1 ≤ x → 0 ≤ n → 1 ≤ x ^ n.
+Proof with auto using semirings.precedes_0_1.
+  intros E1 E2.
+  pattern n. apply integers.induction_nonneg...
+    intros ? ? E. now rewrite E...
+   now rewrite int_pow_0.
+  intros ? E3 E4.
+  rewrite int_pow_S.
+   rewrite <-rings.mult_1_r.
+   apply semirings.nonneg_mult_compat_both...
+  apply not_symmetry, orders.neq_precedes_sprecedes.
+  apply orders.sprecedes_trans_l with 1...
+  now apply semirings.sprecedes_0_1.
+Qed.
+
+Lemma int_pow_exp_precedes (x : A) (n m : B) : 1 ≤ x → n ≤ m → x ^ n ≤ x ^ m.
+Proof.
+  intros ? E2.
+  assert (0 < x) as [? ?]. 
+   apply orders.sprecedes_trans_l with 1.
+    now apply semirings.sprecedes_0_1.
+   easy.
+  apply srorder_plus in E2. destruct E2 as [z [E2a E2b]].
+  rewrite E2b.
+  rewrite int_pow_exp_plus.
+   rewrite <-rings.mult_1_r.
+   apply semirings.nonneg_mult_compat_both.
+      now apply int_pow_nonneg.
+     apply semirings.precedes_0_1.
+    now ring_simplify.
+   now apply int_pow_ge1.
+   now apply not_symmetry.
+Qed. 
 End int_pow_properties.
 
 Section preservation.
   Context 
     `{Integers B} `{oB : Order B} `{!RingOrder oB} `{!TotalOrder oB}
-    `{Field A1} `{∀ z : A1, NeZero z → LeftCancellation (.*.) z} `{∀ x y : A1, Decision (x = y)} `{!DecMultInv A1} `{!IntPow A1 B}
-    `{Field A2} `{∀ z : A2, NeZero z → LeftCancellation (.*.) z} `{∀ x y : A2, Decision (x = y)} `{!DecMultInv A2} `{!IntPow A2 B}
+    `{Field A1} `{∀ x y : A1, Decision (x = y)} `{!DecMultInv A1} `{!IntPowSpec A1 B ip1}
+    `{Field A2} `{∀ x y : A2, Decision (x = y)} `{!DecMultInv A2} `{!IntPowSpec A2 B ip2}
     {f : A1 → A2} `{!OrderPreserving f} `{!SemiRing_Morphism f} `{!Injective f}.
 
   Add Ring B2 : (rings.stdlib_ring_theory B).
@@ -226,64 +226,74 @@ Section preservation.
   Lemma preserves_int_pow x (n : B) : f (x ^ n) = (f x) ^ n.
   Proof with auto.
     revert n. apply integers.induction.
-       intros ? ? E1. rewrite E1. reflexivity.
-      rewrite int_pow_0, int_pow_0. apply rings.preserves_1.
+       solve_proper.
+      rewrite int_pow_0, int_pow_0. now apply rings.preserves_1.
      intros n E F. 
      rewrite int_pow_S_nonneg, rings.preserves_mult, F...
-     rewrite int_pow_S_nonneg... reflexivity.
+     now rewrite int_pow_S_nonneg.
     intros n E F.
-    destruct (decide (x = 0)) as [G | G].
+    destruct (decide (x = 0)) as [G|G].
      rewrite G. rewrite rings.preserves_0. 
      assert (n - 1 ≠ 0).
       apply orders.neq_precedes_sprecedes, integers.precedes_sprecedes_alt.
       ring_simplify...
-     repeat rewrite int_pow_of_0...
-     apply rings.preserves_0.
+     repeat rewrite int_pow_base_0...
+     now apply rings.preserves_0.
     assert (f x ≠ 0). apply rings.injective_not_0...
     apply (rings.left_cancellation_ne_0 (.*.) (f x))...
     rewrite <-int_pow_S, <-rings.preserves_mult, <-int_pow_S...
-    setoid_replace (1 + (n - 1)) with n by ring...
+    now setoid_replace (1 + (n - 1)) with n by ring.
   Qed.
 End preservation.
 
 (* Very slow default implementation by translation into Peano *)
 Section int_pow_default.
-  Context `{Field A} 
-    `{∀ z, NeZero z → LeftCancellation (.*.) z}
-    `{∀ x y, Decision (x = y)} `{!DecMultInv A}
+  Context `{Field A} `{∀ x y, Decision (x = y)} `{!DecMultInv A}
     `{Integers B} `{oB : Order B} `{!RingOrder oB} `{!TotalOrder oB}.
 
-  Let int_pow_default (x : A) (n : B) : A := 
+  Add Ring B3 : (rings.stdlib_ring_theory B).
+
+  Global Instance int_pow_default: Pow A B | 10 := λ x n,
     match (decide (0 ≤ n)) with
-    | left _ => x ^ (int_abs B nat n)
-    | right _ => /(x ^ (int_abs B nat n))
+    | left _ => x ^ int_abs B nat n
+    | right _ => /(x ^ int_abs B nat n)
     end.
 
-  Global Program Instance: IntPow A B | 10 := int_pow_default.
-  Next Obligation with try contradiction; auto using semirings.precedes_0_1.
-    apply int_pow_spec_from_properties; unfold int_pow_default.
-       admit.
-      intros y.
-      case (decide _); intros E.
-       rewrite int_abs_0. apply nat_pow_0.
-      destruct E. reflexivity.
-     intros y m E.
-     case (decide _); case (decide _); intros E1 E2...
-      rewrite int_abs_nonneg_plus, int_abs_1...
-      apply nat_pow_S.
+  Global Instance: IntPowSpec A B int_pow_default.
+  Proof with try contradiction; auto using semirings.precedes_0_1.
+    split; unfold pow, int_pow_default.
+       intros ? ? E1 ? ? E2.
+       now (case (decide _); case (decide _); rewrite E1, E2)...
+      intros x. case (decide _); intros E.
+      rewrite int_abs_0. 
+       now apply nat_pow_0.
+      now destruct E.
+     intros n ?. case (decide _); intros E.
+      now apply nat_pow_base_0, int_abs_nonzero.
+     rewrite nat_pow_base_0. 
+     apply fields.dec_mult_inv_0.
+     now apply int_abs_nonzero.
+    intros x n E. case (decide _); case (decide _); intros E1 E2.
+       rewrite int_abs_nonneg_plus, int_abs_1...
+       now rewrite nat_pow_S.
+      setoid_replace n with (-(1):B).
+       rewrite rings.plus_opp_r, int_abs_0, nat_pow_0. 
+       rewrite int_abs_opp, int_abs_1, right_identity. 
+       symmetry. now apply fields.dec_mult_inverse.
+      apply (antisymmetry (≤)).
+       apply orders.not_precedes_sprecedes in E1.
+       apply integers.precedes_sprecedes_alt in E1. 
+       apply (order_preserving_back (+1)).
+       unfold flip. ring_simplify...
+      apply (order_preserving_back (1+)). now rewrite rings.plus_opp_r.
      destruct E2. apply semirings.nonneg_plus_compat_l...
-    intros y m.
-    case (decide _); case (decide _); intros E1 E2...
-       setoid_replace m with (0 : B).
-        rewrite rings.opp_0, int_abs_0, nat_pow_0. symmetry. apply fields.dec_mult_inv_1.
-       apply (antisymmetry (≤))... apply rings.flip_nonpos_inv...
-      rewrite fields.dec_mult_inv_involutive, int_abs_opp. reflexivity.
-     rewrite int_abs_opp. reflexivity.
-    setoid_replace m with (0 : B).
-     rewrite rings.opp_0, int_abs_0, nat_pow_0. rewrite fields.dec_mult_inv_1 at 2. reflexivity.
-    apply (antisymmetry (≤)).
-     apply orders.precedes_flip...
-    apply rings.flip_nonneg_inv.
-    apply orders.precedes_flip...
+     rewrite <-int_abs_opp, <-(int_abs_opp n).
+     setoid_replace (-n) with (1 - (1 + n)) by ring.
+     rewrite (int_abs_nonneg_plus 1 (-(1 + n))), int_abs_1...
+      rewrite nat_pow_S. 
+      rewrite fields.dec_mult_inv_distr, associativity.
+      now rewrite fields.dec_mult_inverse, left_identity...
+     apply rings.flip_nonpos_inv.
+     now apply orders.not_precedes_sprecedes.
   Qed.
 End int_pow_default.
